

# COMP 584 — Homework 1

Dev Sanghvi

NetID: ds221

February 8, 2026

## Problem 1 (20 pts): Text Representation (BoW and TF-IDF)

**Vocabulary (fixed order):**

$\mathcal{V} = [\text{lecture}, \text{homework}, \text{exam}, \text{student}, \text{grade}, \langle \text{unk} \rangle]$

**Documents:**

- $d_1$ : lecture homework homework quiz
- $d_2$ : exam grade grade student
- $d_3$ : student lecture exam

**Tokenization rule:** Split on whitespace. Any token not in  $\mathcal{V}$  is mapped to  $\langle \text{unk} \rangle$ .

### Part I (12 pts): Bag-of-Words (Binary vs. Count)

#### 1. (4 pts) Binary BoW vector for document $d_1$ :

Tokens in  $d_1$ : [lecture, homework, homework, quiz]

Mapping:

- “lecture”  $\in \mathcal{V} \Rightarrow$  index 0
- “homework”  $\in \mathcal{V} \Rightarrow$  index 1
- “quiz”  $\notin \mathcal{V} \Rightarrow$  maps to  $\langle \text{unk} \rangle$  at index 5

**Binary BoW** (1 if token appears at least once, 0 otherwise):

$$\mathbf{x}_{d_1}^{\text{binary}} = [1, 1, 0, 0, 0, 1]$$

#### 2. (4 pts) Count BoW vector for document $d_1$ :

Token counts:

- lecture: 1
- homework: 2
- quiz  $\rightarrow \langle \text{unk} \rangle$ : 1

$$\mathbf{x}_{d_1}^{\text{count}} = [1, 2, 0, 0, 0, 1]$$

#### 3. (4 pts) Count BoW vector for document $d_2$ :

Tokens in  $d_2$ : [exam, grade, grade, student]

Token counts:

- exam: 1

- grade: 2
- student: 1

$$\mathbf{x}_{d_2}^{\text{count}} = [0, 0, 1, 1, 2, 0]$$

## Part II (8 pts): TF-IDF

$N = 3$  documents in the corpus.

1. (4 pts) Compute  $\text{df}(t)$  for each token  $t \in \mathcal{V}$ :

Token	Appears in	df( $t$ )
lecture	$d_1, d_3$	2
homework	$d_1$	1
exam	$d_2, d_3$	2
student	$d_2, d_3$	2
grade	$d_2$	1
$\langle \text{unk} \rangle$	$d_1$ (from “quiz”)	1

$$\text{df} = [2, 1, 2, 2, 1, 1]$$

2. (4 pts) TF-IDF vector for document  $d_1$ :

Recall:  $\text{idf}(t) = \ln\left(\frac{N}{\text{df}(t)}\right)$  and  $\text{tf-idf}(t, d) = \text{tf}(t, d) \cdot \text{idf}(t)$ .

Token	tf( $t, d_1$ )	idf( $t$ )	tf · idf
lecture	1	$\ln(3/2)$	$\ln(3/2)$
homework	2	$\ln(3/1) = \ln 3$	$2 \ln 3$
exam	0	$\ln(3/2)$	0
student	0	$\ln(3/2)$	0
grade	0	$\ln 3$	0
$\langle \text{unk} \rangle$	1	$\ln 3$	$\ln 3$

$$\mathbf{x}_{d_1}^{\text{tf-idf}} = [\ln \frac{3}{2}, 2 \ln 3, 0, 0, 0, \ln 3]$$

## Problem 2 (30 pts): Classification

Throughout this problem, consider a single training example  $(\mathbf{x}, y)$  with  $y \in \{0, 1\}$ , and use the sigmoid function  $\sigma(z) = \frac{1}{1+e^{-z}}$ .

### Part I (12 pts): A Simple Two-Layer MLP

Model:

$$\mathbf{h} = W^{(1)}\mathbf{x}, \quad z = \mathbf{w}^{(2)\top}\mathbf{h} + b, \quad \hat{y} = \sigma(z)$$

Loss:

$$\mathcal{L} = -[y \log \hat{y} + (1 - y) \log(1 - \hat{y})]$$

#### 1. (5 pts) Why maximize log-likelihood instead of likelihood?

- (a) **Numerical Stability:** Likelihoods are products of probabilities, which can become extremely small (underflow) for large datasets. Taking the logarithm converts products into sums, preventing numerical underflow.
- (b) **Convexity:** For many models (e.g., logistic regression), the log-likelihood is a concave function of the parameters, making optimization easier with gradient-based methods. The raw likelihood is not convex.
- (c) **Gradient Simplicity:** Derivatives of log-likelihoods often have simpler, cleaner forms. For example, gradients involve  $(y - \hat{y})$  terms rather than complex products.

#### 2. (7 pts) Derive negative log-likelihood for $y \sim \text{Bernoulli}(\hat{y})$ :

The Bernoulli probability mass function is:

$$P(y \mid \hat{y}) = \hat{y}^y (1 - \hat{y})^{1-y}$$

Taking the log:

$$\log P(y \mid \hat{y}) = y \log \hat{y} + (1 - y) \log(1 - \hat{y})$$

The negative log-likelihood (NLL) is:

$$\mathcal{L} = -\log P(y \mid \hat{y}) = -[y \log \hat{y} + (1 - y) \log(1 - \hat{y})]$$

$$\mathcal{L} = -y \log \hat{y} - (1 - y) \log(1 - \hat{y})$$

This is exactly the **binary cross-entropy loss**.

### Part II (4 pts): Forward Pass

Given model:

$$\begin{aligned} \mathbf{a}_1 &= W_1 \mathbf{x} \\ \mathbf{a}_{21} &= W_{21} \mathbf{a}_1, \quad \mathbf{a}_{22} = W_{22} \mathbf{a}_1 \\ \mathbf{a}_2 &= \mathbf{a}_{21} + \mathbf{a}_{22} \\ a_3 &= \mathbf{w}_3^\top \mathbf{a}_2, \quad a_u = \mathbf{u}^\top \mathbf{x} \\ z &= a_3 + a_u, \quad \hat{y} = \sigma(z) \end{aligned}$$

Substituting:

$$\begin{aligned}\mathbf{a}_2 &= W_{21}W_1\mathbf{x} + W_{22}W_1\mathbf{x} = (W_{21} + W_{22})W_1\mathbf{x} \\ a_3 &= \mathbf{w}_3^\top (W_{21} + W_{22})W_1\mathbf{x} \\ z &= \mathbf{w}_3^\top (W_{21} + W_{22})W_1\mathbf{x} + \mathbf{u}^\top \mathbf{x}\end{aligned}$$

$$\hat{y} = \sigma \left( \mathbf{w}_3^\top (W_{21} + W_{22})W_1\mathbf{x} + \mathbf{u}^\top \mathbf{x} \right)$$

### Part III (7 pts): Backward Pass

Using the chain rule with  $\mathcal{L} = -[y \log \hat{y} + (1 - y) \log(1 - \hat{y})]$ .

First, useful derivative:

$$\frac{\partial \mathcal{L}}{\partial z} = \hat{y} - y$$

**Gradient w.r.t.  $\mathbf{u}$ :**

Since  $z = a_3 + \mathbf{u}^\top \mathbf{x}$ :

$$\frac{\partial z}{\partial \mathbf{u}} = \mathbf{x}$$

$$\frac{\partial \mathcal{L}}{\partial \mathbf{u}} = (\hat{y} - y)\mathbf{x}$$

**Gradient w.r.t.  $W_1$ :**

Chain rule through the network:

$$\frac{\partial \mathcal{L}}{\partial W_1} = \frac{\partial \mathcal{L}}{\partial z} \cdot \frac{\partial z}{\partial \mathbf{a}_2} \cdot \frac{\partial \mathbf{a}_2}{\partial \mathbf{a}_1} \cdot \frac{\partial \mathbf{a}_1}{\partial W_1}$$

Where:

- $\frac{\partial z}{\partial \mathbf{a}_2} = \mathbf{w}_3$
- $\frac{\partial \mathbf{a}_2}{\partial \mathbf{a}_1} = W_{21}^\top + W_{22}^\top = (W_{21} + W_{22})^\top$
- $\frac{\partial \mathbf{a}_1}{\partial W_1} = \mathbf{x}^\top$

$$\frac{\partial \mathcal{L}}{\partial W_1} = (\hat{y} - y)(W_{21} + W_{22})^\top \mathbf{w}_3 \mathbf{x}^\top$$

### Part IV (7 pts): Backward Pass with $W_{\text{super}}$

Modified model:

$$\mathbf{a}_{21} = W_{21}W_{\text{super}}\mathbf{a}_1, \quad \mathbf{a}_{22} = W_{22}W_{\text{super}}\mathbf{a}_1$$

**1. Gradient w.r.t.  $W_{\text{super}}$ :**

Let  $\mathbf{a}_s = W_{\text{super}}\mathbf{a}_1$ . Then  $\mathbf{a}_2 = (W_{21} + W_{22})\mathbf{a}_s$ .

$$\frac{\partial \mathcal{L}}{\partial W_{\text{super}}} = \frac{\partial \mathcal{L}}{\partial z} \cdot \frac{\partial z}{\partial \mathbf{a}_2} \cdot \frac{\partial \mathbf{a}_2}{\partial \mathbf{a}_s} \cdot \frac{\partial \mathbf{a}_s}{\partial W_{\text{super}}}$$

$$\frac{\partial \mathcal{L}}{\partial W_{\text{super}}} = (\hat{y} - y)(W_{21} + W_{22})^\top \mathbf{w}_3 \mathbf{a}_1^\top$$

**2. Gradient w.r.t.  $W_1$ :**

Now the chain extends through  $W_{\text{super}}$ :

$$\frac{\partial \mathcal{L}}{\partial W_1} = (\hat{y} - y) W_{\text{super}}^\top (W_{21} + W_{22})^\top \mathbf{w}_3 \mathbf{x}^\top$$